{
 "cells": [
  {
   "cell_type": "markdown",
   "metadata": {},
   "source": [
    "<span style=\"font-size: 14pt\">EREVAN, May-June 2017</span>\n",
    "\n",
    "<span style=\"font-size: 16pt\"> Seminar #2: Exponential smoothing models\n",
    "\n",
    "<span style=\"color:blue; font-size: 12pt\">Alexey Romanenko </span>,\n",
    "<span style=\"color:blue; font-size: 12pt; font-family: 'Verdana'\">alexromsput@gmail.com</span>\n",
    "\n",
    "\n",
    "<h1 align=\"center\"> Home Work 1 </h1>\n",
    "\n",
    "## Answer questions\n",
    "\n",
    "1) ** How do adaptive properties of SES change when smoothing parameter $\\alpha$ converges to 1?**\n",
    "\n",
    "1) This means that we're giving a greater weight to the last data points in out TS. We choose $\\alpha$ close to 1 when we have trend in our TS, when TS is non-stationary. This will help the model to catch the trend pretty fast, faster then in case of paying too muh attention to the old data points. \n",
    "\n",
    "2) ** What will be the optimal value of smoothing parameter of trend $\\beta$ in Hold model for 1) time series with slowly  changing trend; 2) stochastic changing trend (look <a href=\"http://stochastictrend.blogspot.am/\">here </a>)? **\n",
    "\n",
    "2) 1. For a slower changing trend we will choose $\\beta$ to be close to 0, because we can take into account all the previous data points with almost equal weight. 2. On the other hand in case of a stochastic changing trend we need to choose $\\beta$ closer to 1, so that the recent data points have greater weights and the model is able to catch the fastly changing trend. \n",
    "\n",
    "3) **Proof the equivalency of correction error form and smoothing form for unobserved component of TS in  Thei-Wage model (period of seasonality equals $p$):**\n",
    "\n",
    "  $$l_t = \\alpha (y_t - s_{t-p}) + (1-\\alpha) (l_{t-1} + b_{t-1} )=l_{t-1} + b_{t-1} + \\alpha e_t;$$\n",
    "  $$ b_t = \\beta (l_{t} - l_{t-1} ) + (1-\\beta) b_{t-1} = b_{t-1} + \\alpha\\beta e_t;$$\n",
    "  $$ s_t = \\gamma (y_t-l_t) + (1-\\gamma) s_{t-p} = s_{t-p} + \\gamma(1-\\alpha)e_t.$$\n",
    "  \n",
    "3) We get:\n",
    "\n",
    "  $$ l_t = \\alpha (y_t - s_{t-p}) + (1-\\alpha) (l_{t-1} + b_{t-1} ) = \\alpha (e_t + l_{t-1} + b_{t-1} + s_{t-p} - s_{t-p}) + (1-\\alpha) (l_{t-1} + b_{t-1} ) = l_{t-1} + b_{t-1} + \\alpha e_t. $$\n",
    "  \n",
    "Because we know that:\n",
    "  $$ \\hat{y}_{t|t-1} = l_{t-1} + b_{t-1} + s_{t-p};$$\n",
    "  $$ e_t = y_t - \\hat{y}_{t|t-1} = y_t - l_{t-1} + b_{t-1} + s_{t-p};$$\n",
    "  thus $$y_t = e_t + l_{t-1} + b_{t-1} + s_{t-p}.$$  \n",
    "  \n",
    "Now we have that $l_t = l_{t-1} + b_{t-1} + \\alpha e_t$, so, using the expression obtained for $l_t$ we can get:\n",
    "\n",
    "$$ b_t = \\beta (l_{t} - l_{t-1} ) + (1-\\beta) b_{t-1} = \\beta (l_{t-1} + b_{t-1} + \\alpha e_t - l_{t-1} ) + (1-\\beta) b_{t-1} = b_{t-1} + \\alpha\\beta e_t.$$\n",
    "\n",
    "Also,\n",
    "$$ s_t = \\gamma (y_t-l_t) + (1-\\gamma) s_{t-p} = \\gamma ((e_t + l_{t-1} + b_{t-1} + s_{t-p})-(l_{t-1} + b_{t-1} + \\alpha e_t)) + (1-\\gamma) s_{t-p} = s_{t-p} + \\gamma(1-\\alpha)e_t.$$\n",
    "\n",
    "Since we have obtained new expressions for $l_t$ and $y_t$.\n",
    "\n",
    "\n",
    "4) **Find the correction error form for unobserved component of TS in ES with additive damped trend:**\n",
    "\n",
    "$$\\hat{y}_{t+d|t} = l_t + \\left(\\phi + \\phi^2 + \\dots + \\phi^{d}\\right) b_t.$$\n",
    "\n",
    "**Unobserved components are (in smoothing form): **\n",
    "\n",
    "$$ l_t       = \\alpha y_t + \\left(1-\\alpha\\right) \\left(l_{t-1} +\\phi b_{t-1}\\right),$$\n",
    "$$ b_t         = \\beta \\left(l_t - l_{t-1}\\right) + \\left(1-\\beta\\right)\\phi b_{t-1}.$$\n",
    "\n",
    "\n",
    "4) $$ l_t = \\alpha y_t + \\left(1-\\alpha\\right) \\left(l_{t-1} +\\phi b_{t-1}\\right) = \\alpha (e_t + l_{t-1} + \\phi b_{t-1}) + \\left(1-\\alpha\\right) \\left(l_{t-1} +\\phi b_{t-1}\\right) = \\alpha e_t + l_{t-1} +\\phi b_{t-1}. $$\n",
    "\n",
    "Because similar to $\\hat{y}_{t+d|t}$, we can get that:\n",
    "\n",
    "$$\\hat{y}_{t|t-1} = l_{t-1} + \\phi b_{t-1};$$\n",
    "$$ e_t = y_t - \\hat{y}_{t|t-1} = y_t - l_{t-1} + \\phi b_{t-1};$$\n",
    "thus\n",
    "$$y_t = e_t + l_{t-1} + \\phi b_{t-1} .$$\n",
    "\n",
    "Now that we have a new expression for $l_t$, we can get a new expression for $b_t$ by a simple substitution:\n",
    "\n",
    "$$ b_t = \\beta \\left(l_t - l_{t-1}\\right) + \\left(1-\\beta\\right)\\phi b_{t-1} = \\beta \\left(\\alpha e_t + l_{t-1} +\\phi b_{t-1} - l_{t-1}\\right) + \\left(1-\\beta\\right)\\phi b_{t-1} = \\beta \\alpha e_t + \\phi b_{t-1}.$$"
   ]
  }
 ],
 "metadata": {
  "anaconda-cloud": {},
  "kernelspec": {
   "display_name": "Python 3",
   "language": "python",
   "name": "python3"
  },
  "language_info": {
   "codemirror_mode": {
    "name": "ipython",
    "version": 3
   },
   "file_extension": ".py",
   "mimetype": "text/x-python",
   "name": "python",
   "nbconvert_exporter": "python",
   "pygments_lexer": "ipython3",
   "version": "3.6.1"
  }
 },
 "nbformat": 4,
 "nbformat_minor": 1
}
